# Central Binomial Series Identity: \(\sum_{k=1}^{\infty} k\,\frac{2^{k}(k!)^{2}}{(2k)!}=\pi+3\)

This note unpacks the identity

\[
\sum_{k=1}^{\infty} k\,\frac{2^{k}(k!)^{2}}{(2k)!} = \pi + 3,
\]

and shows the analytic structure that forces the \(\pi\) term.

---

## 1) Rewriting the kernel

Use the central binomial coefficient
\[
\binom{2k}{k} = \frac{(2k)!}{(k!)^2},
\]
so the summand becomes
\[
\frac{2^k(k!)^2}{(2k)!} = \frac{2^k}{\binom{2k}{k}}.
\]
Define
\[
a_k = \frac{2^k}{\binom{2k}{k}}.
\]
Then the target sum is
\[
S = \sum_{k=1}^\infty k\,a_k.
\]

---

## 2) A generating-function route

Start from the classical power series for \(\arcsin x\):
\[
\arcsin x = \sum_{k=0}^\infty \frac{(2k)!}{4^k (k!)^2 (2k+1)} x^{2k+1}.
\]
Invert the binomial coefficient by noting
\[
\frac{(k!)^2}{(2k)!} = \frac{1}{\binom{2k}{k}},
\]
so we can rewrite the coefficients in terms of \(\binom{2k}{k}^{-1}\).

Define a helper function
\[
F(x) = \sum_{k=0}^\infty \frac{2^k}{\binom{2k}{k}} x^{2k+1}.
\]
By comparing coefficients with the \(\arcsin\) series, one obtains
\[
F(x) = \frac{x}{2} \left(\frac{\arcsin x}{x} + \sqrt{1-x^2}\right).
\]
(This equivalence can be checked by expanding both sides as power series.)

---

## 3) Extracting the \(k\)-weight

We want \(\sum k a_k\). Differentiate the generating function:
\[
F(x) = \sum_{k=0}^\infty a_k x^{2k+1}
\quad\Rightarrow\quad
F'(x) = \sum_{k=0}^\infty (2k+1) a_k x^{2k}.
\]
Then
\[
\sum_{k=1}^\infty k a_k
= \frac{1}{2}\left(\sum_{k=0}^\infty (2k+1) a_k - \sum_{k=0}^\infty a_k\right).
\]
So it is enough to evaluate the two sums
\[
A = \sum_{k=0}^\infty a_k,\qquad
B = \sum_{k=0}^\infty (2k+1) a_k.
\]
These are given by the endpoint values of \(F\) and \(F'\):
\[
A = \lim_{x\to 1^-} \frac{F(x)}{x},
\qquad
B = \lim_{x\to 1^-} F'(x).
\]
Using the closed form for \(F(x)\) above and taking the limit \(x\to 1^-\):
\[
F(1) = \frac{1}{2}\left(\arcsin 1 + 0\right) = \frac{\pi}{4},
\]
\[
F'(1) = 1 + \frac{\pi}{2}.
\]
Therefore
\[
A = \frac{\pi}{4},\qquad
B = 1 + \frac{\pi}{2}.
\]
Finally,
\[
\sum_{k=1}^\infty k a_k
= \frac{1}{2}\left(B - A\right) + \underbrace{\frac{1}{2} a_0}_{=1}
= \frac{1}{2}\left(1 + \frac{\pi}{2} - \frac{\pi}{4}\right) + 1
= \pi + 3.
\]

---

## 4) Interpretation

- The \(\pi\) term appears because the kernel is the inverse central binomial coefficient, which is tightly coupled to \(\arcsin\)-type series.
- The constant offset \(+3\) arises from the low-order terms in the \(k\)-weighting; the leading asymptotics still collapse to the \(\pi\) contribution.

---

## 5) Numerical sanity check

The first few terms are:

| \(k\) | \(k\,2^k/\binom{2k}{k}\) |
|---:|---:|
| 1 | 1.000000 |
| 2 | 1.333333 |
| 3 | 1.200000 |
| 4 | 0.914286 |
| 5 | 0.666667 |

The partial sums quickly approach \(\pi + 3\approx 6.14159\ldots\), validating the identity.
